port examples using APC

mutsum/MutAll.v
@@ -1,114 +1,117 @@
 Require Import CRIS Cancel.
-
 Require Import MutHeader MutFA MutGA MutMainA.
 Require Import MutFI MutGI MutMainI.
 Require Import MutFIAproof MutGIAproof MutMainIAproof.
 Require Import APCHeader APC APCI APCA APCC.
 Require Import APCIAproof APCACproof.
 
-Module MutAll.
-  Import inv_instances.
-
-  Local Instance Γ : HRA := ##[invΓ].
-  Local Instance Σ : GRA := ##[Γ; invΣ].
-  Definition irΓ : Γ := **[ir_invΓ].
-  Definition irΣ : Σ := **[irΓ; ir_invΣ].
-
-  Lemma irΣ_valid : ✓ (irΣ ⋅ ir_own_admin).
-  Proof. solve_ir_valid. Qed.
+Section MutAll.
+  Context `{!crisG Γ Σ α β τ Hsub Hinv, !concGS}.
 
   Local Definition smod_src : SMod.t := MutMainA.smod false ☆ MutFA.smod ☆ MutGA.smod ☆ APCC.smod.
-  Local Definition sp : sp_type := sp_from smod_src.
+  Local Definition sp : specmap := SMod.conc_sp_from smod_src.
 
   Local Definition smod_pure : SMod.t := MutFA.smod ☆ MutGA.smod.
-  Local Definition sp_pure : spl_type := MutFA.SpF ++ MutGA.SpG.
+  Local Definition sp_pure : specmap := MutFA.SpF ∪ MutGA.SpG.
 
-  Local Definition mod_top : Mod.t := SMod.to_mod sp_none (SMod.cancel smod_src).
+  Local Definition mod_top : Mod.t := SMod.to_mod ∅ (SMod.cancel smod_src).
   Local Definition mod_src : Mod.t := SMod.to_mod sp smod_src.
   Local Definition mod_tgt : Mod.t := MutMainI.t ★ MutFI.t ★ MutGI.t ★ APCI.t.
 
-  Local Definition init_cond : iProp Σ :=
-    winv (⊤,⊤) ∗ MutFA.init_cond ∗ MutGA.init_cond.
-
   (* Apply cancellation to linked spec module *)
   Lemma cancel_src :
-    refines (mod_top, init_cond)
-            ((mod_src, init_cond) : Mod.modc).
+    refines (mod_top, emp ∗ TID 0 ∗ YIELD 0 ∗ winv (⊤, ⊤) ∗ emp ∗ TIDAUTH 0 ∗ YIELDAUTH 1)%I
+            (mod_src, emp%I).
   Proof.
     eapply Cancel.cancellation.
-    - ii; des; subst; inv FIND; ss; rewrite !eq_rel_dec_correct in H0; des_ifs.
-    - econs; [refl|]; i; inv NS; des; inv H; des; inv H1;
-      rewrite !eq_rel_dec_correct in H2; des_ifs.
-    - econs; unfold_mod; ss; prove_nodup.
+    { repeat apply SMod.cancellable_add; r; mod_tac ss. }
+    { assert (Ht : SMod.conc_sp_from smod_src !! speckey_entry =
+        fsp_none); last (rewrite Ht; clear Ht).
+      { rewrite lookup_insert_ne // lookup_kmap_None. i; ss.
+        rewrite /SMod.lift_fn in H0. des_ifs. }
+      eexists _, _; splits.
+      { ss; exists (tt); split; refl. }
+      { iIntros "[? [? ?]]"; ss. }
+      { unfold_pre_post. iIntros "% % $ //". }
+    }
   Qed.
 
+  Lemma apc_in_sp : APCA.sp ⊆ sp.
+  Proof.
+    repeat try eapply insert_subseteq_l; last apply map_empty_subseteq;
+      rewrite lookup_insert_ne // lookup_kmap_Some; eexists (Some _); split; ss.
+  Qed.
+
+  Lemma mutf_in_pure : MutFA.SpF ⊆ sp_pure.
+  Proof.
+    repeat try eapply insert_subseteq_l; last apply map_empty_subseteq.
+    rewrite /sp_pure lookup_union. simpl_map. rewrite lookup_insert_ne //.
+  Qed.
+
+  Lemma mutg_in_pure : MutGA.SpG ⊆ sp_pure.
+  Proof.
+    repeat try eapply insert_subseteq_l; last apply map_empty_subseteq.
+    rewrite /sp_pure lookup_union. simpl_map. rewrite lookup_insert_ne //.
+  Qed.
+
+  Lemma pure_in_sp : sp_pure ⊆ sp.
+  Proof.
+    rewrite /sp_pure. eapply (map_union_least MutFA.SpF MutGA.SpG); try refl.
+    - repeat try eapply insert_subseteq_l; last apply map_empty_subseteq;
+        rewrite lookup_insert_ne // lookup_kmap_Some; eexists (Some _); split; ss.
+    - repeat try eapply insert_subseteq_l; last apply map_empty_subseteq;
+        rewrite lookup_insert_ne // lookup_kmap_Some; eexists (Some _); split; ss.
+  Qed.
+  
   (* Refinement between spec/impl of whole program (linked module) *)
-  Lemma src_tgt : refines (mod_src, init_cond) (mod_tgt, emp%I).
+  Lemma src_tgt : refines (mod_src, emp%I) (mod_tgt, emp%I).
   Proof.
     eapply ctxr_refines.
-    rewrite /mod_src /mod_tgt !add_interp_comm.
+    rewrite /mod_src /mod_tgt !SMod.to_mod_add.
 
     (* abstraction of APCI to APCA *)
     etrans; cycle 1.
-    { do 3 ctxr_drop.
-      eapply APCIA.ctxr.
-    }
+    { do 3 ctxr_drop. eapply APCIA.ctxr. }
 
     (* abstraction of MutF *)
     etrans; cycle 1.
     { ctxr_drop. ctxr_rotate. ctxr_drop. ctxr_rotate.
       eapply MutFIA.ctxr with (Sp:=sp) (SpPure:=sp_pure).
-      { rewrite /sp /sp_incl /APCA.Sp. unseal CRIS.
-        split; try prove_nodup.
-        i. des_ifs; ss; unfold dec, option_Dec, AList.option_Dec_obligation_1 in *; des_ifs. }
-      { rewrite /sp_pure /MutGA.SpG /spl_sub /MutFA.SpF. unseal CRIS.
-        i. eapply alist_find_comm; try prove_nodup; eapply alist_find_app; eauto. }
-      { rewrite /sp_pure /sp /sp_incl /MutFA.SpF /MutGA.SpG /sp_from. unseal CRIS.
-        split; try prove_nodup. i; ss. des_ifs;
-        i; des_ifs; ss; unfold dec, option_Dec, AList.option_Dec_obligation_1 in *; des_ifs. }
+      { eapply apc_in_sp. }
+      { eapply mutg_in_pure. }
+      { eapply pure_in_sp. }
     }
 
     (* abstraction of MutG *)
     etrans; cycle 1.
     { ctxr_drop. ctxr_rotate. ctxr_drop. ctxr_rotate.
       eapply MutGIA.ctxr with (Sp:=sp) (SpPure:=sp_pure).
-      { rewrite /sp /sp_incl /APCA.Sp. unseal CRIS.
-        split; try prove_nodup.
-        i. des_ifs; ss; unfold dec, option_Dec, AList.option_Dec_obligation_1 in *; des_ifs. }
-      { rewrite /sp_pure /MutGA.SpG /spl_sub /MutFA.SpF. unseal CRIS.
-        i. eapply alist_find_app; eauto. }
-      { rewrite /sp_pure /sp /sp_incl /MutFA.SpF /MutGA.SpG /sp_from. unseal CRIS.
-        split; try prove_nodup. i; ss. des_ifs;
-        i; des_ifs; ss; unfold dec, option_Dec, AList.option_Dec_obligation_1 in *; des_ifs. }
+      { eapply apc_in_sp. }
+      { eapply mutf_in_pure. }
+      { eapply pure_in_sp. }
     }
 
     (* abstraction of MutMain *)
     etrans; cycle 1.
     { ctxr_rotate. do 2 ctxr_drop. ctxr_rotate.
       eapply MutMainIA.ctxr with (Sp:=sp) (SpPure:=sp_pure).
-      { rewrite /sp /sp_incl /APCA.Sp. unseal CRIS.
-        split; try prove_nodup.
-        i. des_ifs; ss; unfold dec, option_Dec, AList.option_Dec_obligation_1 in *; des_ifs. }
-      { rewrite /sp_pure /MutGA.SpG /spl_sub /MutFA.SpF. unseal CRIS.
-        i. eapply alist_find_app; eauto. }
-      { rewrite /sp_pure /sp /sp_incl /MutFA.SpF /MutGA.SpG /sp_from. unseal CRIS.
-        split; try prove_nodup. i; ss. des_ifs;
-        i; des_ifs; ss; unfold dec, option_Dec, AList.option_Dec_obligation_1 in *; des_ifs. }
+      { eapply apc_in_sp. }
+      { eapply mutf_in_pure. }
+      { eapply pure_in_sp. }
     }
     
     (* abstraction of APCA to APCC *)
     etrans; cycle 1.
     { do 2 ctxr_rotate. ctxr_drop. eapply APCAC.ctxr.
-      { rewrite /sp /sp_incl /APCA.Sp. unseal CRIS.
-        split; try prove_nodup.
-        i. des_ifs; ss; unfold dec, option_Dec, AList.option_Dec_obligation_1 in *; des_ifs. }
-      { rewrite /sp_pure /sp /sp_incl /MutFA.SpF /MutGA.SpG /sp_from. unseal CRIS.
-        split; try prove_nodup. i; ss. des_ifs;
-        i; des_ifs; ss; unfold dec, option_Dec, AList.option_Dec_obligation_1 in *; des_ifs. }
-      { rewrite /sp_pure /MutFA.SpF /MutGA.SpG /find_body; unfold_mod.
-        i; ss; des_ifs.
-        { do 2 eexists. unfold_mod; ss; des_ifs. }
-        { do 2 eexists. hrepeat do 2 unfold_mod; ss; des_ifs. }
+      { eapply apc_in_sp. }
+      { eapply pure_in_sp. }
+      { i; ss.
+        rewrite /sp_pure lookup_union in H0.
+        destruct (String.eq_dec fn MutHdr.mutf).
+        { subst. rewrite lookup_insert lookup_insert_ne // lookup_empty in H0. inv H0. esplits; eauto. }
+        destruct (String.eq_dec fn MutHdr.mutg).
+        { subst. rewrite lookup_insert lookup_insert_ne // lookup_empty in H0. inv H0. esplits; eauto. }
+        rewrite !lookup_insert_ne // in H0; ii; inv H0.
       }
     }
 
@@ -116,26 +119,20 @@ Module MutAll.
     etrans; cycle 1.
     { do 2 ctxr_rotate. do 2 ctxr_drop.
       eapply MutMainIA.ctxr_close with (Sp:=sp) (SpPure:=sp_pure).
-      { rewrite /sp /sp_incl /APCA.Sp. unseal CRIS.
-        split; try prove_nodup.
-        i. des_ifs; ss; unfold dec, option_Dec, AList.option_Dec_obligation_1 in *; des_ifs. }
-      { rewrite /sp_pure /MutGA.SpG /spl_sub /MutFA.SpF. unseal CRIS.
-        i. eapply alist_find_app; eauto. }
-      { rewrite /sp_pure /sp /sp_incl /MutFA.SpF /MutGA.SpG /sp_from. unseal CRIS.
-        split; try prove_nodup. i; ss. des_ifs;
-        i; des_ifs; ss; unfold dec, option_Dec, AList.option_Dec_obligation_1 in *; des_ifs. }
+      { eapply apc_in_sp. }
+      { eapply mutf_in_pure. }
+      { eapply pure_in_sp. }
     }
 
     etrans; cycle 1.
     { do 2 ctxr_rotate. ctxr_swap. ctxr_rotate. ctxr_refl. }
 
-    rewrite /MutMainA.t /MutFA.t /MutGA.t /APCC.t. unseal CRIS.
-    eapply ctxr_cond_strengthen.
-    iIntros "[? ?]". iFrame.
+    rewrite /MutMainA.t /MutFA.t /MutGA.t /APCC.t.
+    eapply ctxr_cond_strengthen. eauto.
   (*SLOW*)Qed.
 
   Lemma top_tgt :
-    refines (mod_top, init_cond)
+    refines (mod_top, emp ∗ TID 0 ∗ YIELD 0 ∗ winv (⊤, ⊤) ∗ emp ∗ TIDAUTH 0 ∗ YIELDAUTH 1)%I
             (mod_tgt, emp%I).
   Proof.
     etrans.
@@ -143,34 +140,52 @@ Module MutAll.
     { eapply src_tgt. }
   Qed.
 
-  Lemma tgt_wf:
-    Mod.wf mod_tgt.
+  Lemma tgt_wf : Mod.wf mod_tgt.
   Proof.
-    rewrite /mod_tgt /MutMainI.t /MutFI.t /MutGI.t /APCI.t; unseal CRIS; prove_nodup.    
-  Qed.
-
-  Lemma init_cond_valid:
-    ∃ rs, ✓ rs ∧ (Own rs ⊢ init_cond).
-  Proof.
-    exists (irΣ ⋅ ir_own_admin). split.
-    - apply irΣ_valid.
-    - simplify_res.
-      { rewrite make_own_admin; iFrame.
-        et.
+    rewrite /mod_tgt; eapply Mod.add_wf.
+    { econs; eauto; [mod_tac|prove_nodup]. }
+    { eapply Mod.add_wf.
+      { econs; eauto; [mod_tac|prove_nodup]. }
+      { eapply Mod.add_wf.
+        { econs; eauto; [mod_tac|prove_nodup]. }
+        { econs; eauto; [mod_tac|prove_nodup]. }
+        { set_solver. }
+        { prove_nodup; set_solver. }
       }
-      all: solve_res.
+      { rewrite Mod.dom_fnsems_add; set_solver. }
+      { prove_nodup; set_solver. }
+    }
+    { rewrite !Mod.dom_fnsems_add; set_solver. }
+    { prove_nodup; set_solver. }
   Qed.
+End MutAll.
+
+Module MutAll.
+  Import inv_instances.
+
+  Local Instance Γ : HRA := ##[invΓ; concΓ].
+  Local Instance Σ : GRA := ##[Γ; invΣ].
 
   Theorem behavioral_refinement :
-    ∃ src_res tgt_res, refines_lmod
+    ∃ β τ (Hinv : invGS Γ Σ α) (_ : crisG Γ Σ α β τ _ Hinv) (_ : concGS)
+      src_res tgt_res, refines_lmod
       (Mod.to_lmod mod_top src_res)
       (Mod.to_lmod mod_tgt tgt_res).
   Proof.
-    move: (top_tgt)=>H; rewrite /refines in H; des; ss.
-    hexploit H; eauto using tgt_wf. clear H; intros [WF H].
-    assert (IV:= init_cond_valid). des.
-    destruct (H rs); des; et.
-    rewrite IV0 /init_cond {1}winv_split_empty. iIntros "[[? ?] ?]". iFrame; done.
+    apply own_admin_soundness.
+    iMod winv_alloc as "[% [% [% [% ?]]]]"; iExists _, _, _, _.
+    iMod conc_alloc as "[% ?]"; iExists _.
+    pose proof top_tgt as Href.
+    iStopProof. eapply entails_pointwise; iIntros (res Hres) "R".
+    iPoseProof (Own_valid with "R") as "%".
+    rewrite /refines in Href; hexploit Href; eauto using tgt_wf.
+    clear Href; intros [? Href].
+    iPureIntro; hexploit (Href res); eauto.
+    { rewrite Hres; iIntros "[W ($ & $ & $ & $)]".
+      rewrite {1}winv_split_empty comm //.
+    }
+    intros [rt ?].
+    exists res, rt; by des.
   (*SLOW*)Qed.
 End MutAll.
 (* Print Assumptions MutAll.behavioral_refinement. *)
