mutsum/MutMainA.v
@@ -4,7 +4,7 @@ Require Import MutHeader APCHeader APC.
 Set Implicit Arguments.
 
 Module MutMainA. Section MutMainA.
-  Context `{!crisG Γ Σ α β τ _S _I}.
+  Context `{!crisG Γ Σ α β τ Hinv Hsub, !concGS}.
 
   Variable with_pure: bool.
   
@@ -13,22 +13,21 @@ Module MutMainA. Section MutMainA.
   Definition main_body : Any.t → itree crisE Any.t :=
     λ _, (if with_pure then pure else Ret ()↑);;; Ret (Vint 55)↑.
 
-  Definition Sp: spl_type :=
-    Seal.sealing CRIS [(None, None)].
+  (* Definition Sp: specmap := *)
+  (*   {[speckey_entry := fspec_to_rel fspec_trivial]}. *)
 
-  Definition fnsems : fnsems_type :=
-    [(None, (true, wmask_all, scopes, (None, main_body)))].
+  Definition fnsems : fnsemmap :=
+    {[None := Some (msk_scp scopes msk_true, (None, main_body))]}.
 
   Program Definition smod: SMod.t :=
   {|
     SMod.scopes := scopes;
     SMod.fnsems := fnsems;
-    SMod.initial_st := [];
+    SMod.initial_st := ∅;
   |}.
-  Solve All Obligations with prove_scope.
-  Next Obligation. prove_nodup. Qed.
+  Solve All Obligations with mod_tac.
 
   Definition init_cond : iProp Σ := emp%I.
 
-  Definition t Sp := Seal.sealing CRIS (SMod.to_mod Sp smod).
+  Definition t Sp := SMod.to_mod Sp smod.
 End MutMainA. End MutMainA.
