repeat/RepeatI.v
@@ -5,7 +5,7 @@ Require Import RepeatHeader.
 Set Implicit Arguments.
 
 Module RepeatI. Section RepeatI.
-  Context `{Σ : GRA}.
+  Context `{!crisG Σ Γ α β τ Hinv Hsub, !concGS}.
 
   Definition scopes := [RepeatHdr.mn].
 
@@ -20,16 +20,15 @@ Module RepeatI. Section RepeatI.
         v <- ccallU fn [Vint x];;
         ccallU RepeatHdr.repeat [Vptr (fb, 0%Z); Vint (n - 1); v].
 
-  Definition fnsems (genv: GEnv.t) : fnsems_type :=
-    [(Some RepeatHdr.repeat, (false, wmask_all, scopes, (None, cfunU (repeat (CEnv.load_genv genv: CEnv.t)))))].
+  Definition fnsems (genv: GEnv.t) : fnsemmap :=
+    {[Some RepeatHdr.repeat := Some (msk_scp scopes msk_true, (None, cfunU (repeat (CEnv.load_genv genv: CEnv.t))))]}.
 
   Program Definition smod (genv: GEnv.t) : SMod.t := {|
     SMod.scopes := scopes;
     SMod.fnsems := fnsems genv;
-    SMod.initial_st := [];
+    SMod.initial_st := ∅;
   |}.
-  Solve All Obligations with prove_scope.
-  Next Obligation. prove_nodup. Qed.
+  Solve All Obligations with mod_tac.
 
-  Definition t (genv: GEnv.t) : Mod.t := Seal.sealing CRIS (SMod.to_mod sp_none (smod genv)).
+  Definition t (genv: GEnv.t) : Mod.t := SMod.to_mod ∅ (smod genv).
 End RepeatI. End RepeatI.
