repeat/RepeatIAproof.v
@@ -7,18 +7,17 @@ Set Implicit Arguments.
 
 Module RepeatIA. Section RepeatIA.
   Import RepeatAS APC APCA.
-  Context `{_crisG: !crisG Γ Σ α β τ _S _I}.
+  Context `{!crisG Γ Σ α β τ Hinv Hsub, !concGS}.
 
   Context (genv : GEnv.t).
-  Context (sp : sp_type).
-  Context (sp_pure sp_pure_fun : spl_type). (* sp_pure_fun stores fspecs which repeat use *)
+  Context (sp sp_pure sp_pure_fun : specmap).
 
   (* SPC Hypothesis *)
-  Context (APCInSpPure : spl_sub APCA.Sp sp_pure).
-  Context (SpPureInSp : sp_incl sp_pure sp).
-  Context (SpPureFunInSpPure : spl_sub sp_pure_fun sp_pure).
-  Context (repeatInSpPure : alist_find (Some RepeatHdr.repeat) sp_pure 
-            = Some (fsp_some (RepeatAS.repeat_spec sp_pure_fun genv))). (* to avoid recursive definition of SpPure *)
+  Context (APCInSp : APCA.sp ⊆ sp).
+  Context (SpPureInSp : sp_pure ⊆ sp).
+  Context (SpPureFunInSpPure : sp_pure_fun ⊆ sp_pure).
+  Context (repeatInSpPure : sp_pure !! (speckey_fn RepeatHdr.repeat)
+            = Some (fspec_to_rel (RepeatAS.repeat_spec sp_pure_fun genv))).
 
   (* Modules *)
   Local Definition APCA := (APCA.t sp_pure sp).
@@ -28,23 +27,24 @@ Module RepeatIA. Section RepeatIA.
   Local Definition RepeatAMod := (RepeatA ★ APCA).
 
   (* IST *)
-  Definition Ist : alist key Any.t → alist key Any.t → iProp Σ :=
-    (λ st_src st_tgt, emp%I).
+  Definition Ist : gmap key (option Any.t) → gmap key (option Any.t) → iProp Σ :=
+    (λ _ _, True)%I.
   Local Definition IstFull := (IstProd (IstSB RepeatA.(Mod.scopes) Ist) IstEq).
 
-  Lemma simF_repeat : ISim.sim_fun open RepeatAMod RepeatIMod RepeatA.init_cond IstFull (Some RepeatHdr.repeat).
-  Proof using _crisG APCInSpPure SpPureInSp SpPureFunInSpPure repeatInSpPure.
+  Lemma simF_repeat : ISim.sim_fun open RepeatAMod RepeatIMod IstFull (Some RepeatHdr.repeat).
+  Proof using APCInSp SpPureInSp SpPureFunInSpPure repeatInSpPure.
     (* Simulation Start *)
-    init_simF.
+    iStartSim.
 
     (* SRC: handle the precond of repeat *)
-    steps_l. rename _q2 into f_sem, _q3 into n, _q4 into x.
-    iDestruct "ASM" as "%". hss. dup H3. inv H3. steps_l.
+    steps_l. destruct _q as [[n x] f_sem].
+    iDestruct "ASM" as "%". hss. dup H4. inv H4. rewrite /pure_body /cfunN. hss_l.
+    steps_l.
 
     (* SRC: find apc in sp *)
-    assert (SPAPC: sp APCHdr.apc = fsp_some apc_spec).
-    { apply SpPureInSp. apply APCInSpPure. rewrite /Sp. unseal CRIS. ss. }
-    rewrite SPAPC.
+    assert (SPAPC: sp !! speckey_fn APCHdr.apc = fsp_some apc_spec).
+    { erewrite lookup_weaken; [refl| |eapply APCInSp]. rewrite /APCA.sp; simpl_map; refl. }
+    rewrite SPAPC /=.
 
     (* TGT: handle input *)
     steps_r. unfold assume. force_r. steps_r.
@@ -73,7 +73,7 @@ Module RepeatIA. Section RepeatIA.
     {
       (* TGT: load fn from function pointer *)
       destruct (Z_lt_le_dec (S n') 1) eqn:E; try lia.
-      rewrite H2. hss. steps_r.
+      rewrite H1. hss. steps_r.
 
       (* SRC: unfold APC *)
       forces_l. iSplit; eauto. steps_l. 
@@ -84,7 +84,9 @@ Module RepeatIA. Section RepeatIA.
       apc_call_weaker "IST"; et.
       { instantiate (1:= 1%ord). apply OrdArith.lt_from_nat. lia. }
       { eapply Ord.lt_le_lt; et. apply OrdArith.lt_add_r. instantiate (1:=n'). apply OrdArith.lt_from_nat. lia. }
+      iSplitL "IST".
       { unfold precond. ss. do 2 (iSplit; et). iExists (Ord.omega + n')%ord. iSplit; et. iPureIntro. apply OrdArith.add_base_l. }
+      iIntros (???) "ISTPOST".
       iDestruct "ISTPOST" as "[IST %]". unfold postcond. subst.
 
       (* TGT: steps tgt *)
@@ -97,6 +99,7 @@ Module RepeatIA. Section RepeatIA.
       { unfold precond. ss. iFrame. instantiate (1:= (n', (f_sem x), f_sem)). iPureIntro. split.
         - exists fn, fptr. hrepeat split; et. unfold_intrange_64; des_ifs_safe; hrepeat destruct Z_le_gt_dec; ss; try lia.
         - exists (Ord.omega + n')%ord. split; et. apply Ord.le_refl. }
+      iIntros (???) "ISTPOST".
       unfold postcond. ss.
       iDestruct "ISTPOST" as "[IST %]". subst.
 
@@ -109,25 +112,25 @@ Module RepeatIA. Section RepeatIA.
       (* prove the IST *)
       step. by iSplit.
     }
-    Unshelve. all: et. exact (0↑).
+    Unshelve. all: et. all: exact (0↑). 
   (*SLOW*)Qed.
 
   Theorem sim : ISim.t open RepeatAMod RepeatIMod RepeatA.init_cond IstFull.
   Proof.
     init_sim.
-    - split; eauto. iIntros "_". iModIntro. repeat (iSplit; eauto); iPureIntro; ss.
     - apply simF_repeat; eauto.
+    - iIntros "_". rewrite /IstProd. eauto.
   Qed.
 End RepeatIA. 
 
 Section ctxr.
-  Context `{_crisG: !crisG Γ Σ α β τ _S _I}.
+  Context `{_crisG: !crisG Γ Σ α β τ _S _I, !concGS}.
 
-  Definition ctxr (ge : GEnv.t) (sp : sp_type) (sp_pure sp_pure_fun : spl_type)
-        (APCInSpPure : spl_sub APCA.Sp sp_pure)
-        (SpPureInSp : sp_incl sp_pure sp)
-        (SpPureFunInSpPure : spl_sub sp_pure_fun sp_pure)
-        (repeatInSpPure: alist_find (Some RepeatHdr.repeat) sp_pure = Some (fsp_some (RepeatAS.repeat_spec sp_pure_fun ge))) :
+  Definition ctxr (ge : GEnv.t) (sp sp_pure sp_pure_fun : specmap)
+        (APCInSp : APCA.sp ⊆ sp)
+        (SpPureInSp : sp_pure ⊆ sp)
+        (SpPureFunInSpPure : sp_pure_fun ⊆ sp_pure)
+        (repeatInSpPure: sp_pure !! (speckey_fn RepeatHdr.repeat) = Some (fspec_to_rel (RepeatAS.repeat_spec sp_pure_fun ge))) :
     ctx_refines
       ((RepeatA.t ge sp sp_pure_fun) ★ (APCA.t sp_pure sp), emp%I)
       ((RepeatI.t ge)                    ★ (APCA.t sp_pure sp), emp%I).
